Shorten proofs.

examples/n_german/CMP.thy
@@ -757,6 +757,7 @@ proof -
     using a b by auto
 qed
 
+
 lemma symParamFormForallExcl:
   assumes "symParamForm2 N f"
   shows "symParamForm N (\<lambda>i. forallFormExcl (\<lambda>j. f i j) i N)"
@@ -1018,26 +1019,62 @@ lemma symParamRuleI:
   "symParamForm N f \<Longrightarrow> symParamStatement N ps \<Longrightarrow> symParamRule N (\<lambda>i. guard (f i) (ps i))"
   unfolding symParamRule_def symParamForm_def symParamStatement_def by auto
 
-
+text \<open>A set of rules is symmetric with respect to semantic equivalence\<close>
 definition symProtRules' :: "nat \<Rightarrow> rule set \<Rightarrow> bool" where [simp]:
   "symProtRules' N rs = (\<forall>p r. p permutes {x. x \<le> N} \<and> r \<in> rs \<longrightarrow>
-  (\<exists>r'. r'\<in> rs \<and> equivRule  (applySym2Rule p r) r'))"
+     (\<exists>r'. r' \<in> rs \<and> equivRule (applySym2Rule p r) r'))"
 
- 
+text \<open>A set of formulas is symmetric with respect to semantic equivalence\<close>
 definition symPredSet' :: "nat \<Rightarrow> formula set \<Rightarrow> bool" where [simp]:
-  "symPredSet' N fs = 
-  (\<forall>p f. p permutes {x. x \<le> N} \<and> f \<in> fs \<longrightarrow>(\<exists>f'. f'\<in>fs\<and>equivForm (applySym2Form p f) f'))"
+  "symPredSet' N fs = (\<forall>p f. p permutes {x. x \<le> N} \<and> f \<in> fs \<longrightarrow>
+     (\<exists>f'. f' \<in> fs \<and> equivForm (applySym2Form p f) f'))"
+
+lemma symPredSetForall:
+  assumes "symParamForm N f"
+  shows "symPredSet' N {(\<forall>\<^sub>fi. f i) N}"
+proof -
+  have a: "formEval (f i) s"
+    if "p permutes {x. x \<le> N}" "\<forall>i\<le>N. formEval (applySym2Form p (f i)) s" "i \<le> N" for p i s
+  proof -
+    have 1: "inv p i \<le> N"
+      using that(1,3)
+      by (metis (full_types) mem_Collect_eq permutes_def permutes_inverses(1))
+    have 2: "formEval (applySym2Form p (f (inv p i))) s"
+      using that(2) 1 by auto
+    have 3: "equivForm (applySym2Form p (f (inv p i))) (f i)"
+      using that assms unfolding symParamForm_def
+      using 1 permutes_inverses(1) by fastforce
+    show ?thesis
+      using 2 3 unfolding equivForm_def by auto
+  qed
+  have b: "formEval (applySym2Form p (f i)) s"
+    if "p permutes {x. x \<le> N}" "\<forall>i\<le>N. formEval (f i) s" "i \<le> N" for p i s
+  proof -
+    have 1: "p i \<le> N"
+      using bij_betwE permutes_imp_bij that(1,3) by fastforce
+    have 2: "formEval (f (p i)) s"
+      using that(2) 1 by auto
+    have 3: "equivForm (applySym2Form p (f i)) (f (p i))"
+      using assms that unfolding symParamForm_def by auto
+    show ?thesis
+      using 2 3 unfolding equivForm_def by auto
+  qed
+  show ?thesis
+    unfolding symPredSet'_def equivForm_def
+    using a b by auto
+qed
 
 lemma trans1Symmetric':
   assumes "p permutes {x. x \<le> N}"
-    "equivStatement S' (applySym2Statement p S)"
+    and "equivStatement S' (applySym2Statement p S)"
   shows "applySym2State p (trans1 S s0) = trans1 S' (applySym2State p s0)"
-  using assms(1) assms(2) equivStatement_def trans1Symmetric by auto
+  using assms equivStatement_def trans1Symmetric by auto
 
 lemma stFormSymCorrespondence1':
-  assumes "p permutes {x. x \<le> N}" and "equivForm (applySym2Form p f) f'"
-  shows   "formEval f' (applySym2State p s) = formEval f s"
-  using assms(1) assms(2) equivForm_def stFormSymCorrespondence by blast
+  assumes "p permutes {x. x \<le> N}"
+    and "equivForm (applySym2Form p f) f'"
+  shows "formEval f' (applySym2State p s) = formEval f s"
+  using assms equivForm_def stFormSymCorrespondence by blast
    
 lemma reachSymLemma':
   assumes "symPredSet' N fs"
@@ -1056,51 +1093,33 @@ proof (induction i)
 next
   case (Suc i)
   fix i
-  assume a0:"\<forall>s. reachableUpTo fs rs i s \<longrightarrow> reachableUpTo fs rs i (applySym2State p s) "
-  show "  \<forall>s. reachableUpTo fs rs (Suc i) s \<longrightarrow> reachableUpTo fs rs (Suc i) (applySym2State p s)"
-  proof(rule allI, rule)
+  assume a0: "\<forall>s. reachableUpTo fs rs i s \<longrightarrow> reachableUpTo fs rs i (applySym2State p s) "
+  show "\<forall>s. reachableUpTo fs rs (Suc i) s \<longrightarrow> reachableUpTo fs rs (Suc i) (applySym2State p s)"
+  proof (rule allI, rule)
     fix s
-    assume a1:"reachableUpTo fs rs (Suc i) s"
+    assume a1: "reachableUpTo fs rs (Suc i) s"
     have "\<exists>s0 g a. reachableUpTo fs rs i s0 \<and> formEval g s0 \<and>s=trans1 a s0 \<and> guard g a \<in> rs"
       by (meson a1 reachableUpToSuc)
-    then obtain s0 g a where a2:"reachableUpTo fs rs i s0 \<and> formEval g s0 \<and>s=trans1 a s0 \<and> guard g a \<in> rs"
+    then obtain s0 g a where a2: "reachableUpTo fs rs i s0 \<and> formEval g s0 \<and>s=trans1 a s0 \<and> guard g a \<in> rs"
       by blast
-    have a3:" \<exists>r'. equivRule (guard (applySym2Form p g) (applySym2Statement p a)) r'\<and> r' \<in> rs"
+    have "\<exists>r'. equivRule (guard (applySym2Form p g) (applySym2Statement p a)) r'\<and> r' \<in> rs"
       using a2 assms(2) assms(3) by fastforce 
-    then obtain g' a' where a3:"equivRule (guard (applySym2Form p g) (applySym2Statement p a)) 
-  (guard g' a')\<and> (guard g' a') \<in> rs"
+    then obtain g' a' where a3:
+      "equivRule (guard (applySym2Form p g) (applySym2Statement p a)) (guard g' a') \<and>
+       guard g' a' \<in> rs"
       by (metis equivRule.elims(2))
-    then have a31:"equivForm  (applySym2Form p g) g' \<and>equivStatement (applySym2Statement p a) a'"
+    then have a31: "equivForm  (applySym2Form p g) g' \<and> equivStatement (applySym2Statement p a) a'"
       by auto
-    have a4:"reachableUpTo fs rs i (applySym2State p s0)"
+    have a4: "reachableUpTo fs rs i (applySym2State p s0)"
       using a0 a2 by blast  
-    have a5:"formEval  g' (applySym2State p s0)"
-      using a2 a3 assms(3) stFormSymCorrespondence1' by auto 
-      
-    have a5:"reachableUpTo fs rs (Suc i) (trans1 a' (applySym2State p s0))"
-      using a3 a4 a5 reachableSetNext by blast
-    show " reachableUpTo fs rs (Suc i) (applySym2State p s)"
+    have "formEval g' (applySym2State p s0)"
+      using a2 a3 assms(3) stFormSymCorrespondence1' by auto
+    then have a5: "reachableUpTo fs rs (Suc i) (trans1 a' (applySym2State p s0))"
+      using a3 a4 reachableSetNext by blast
+    show "reachableUpTo fs rs (Suc i) (applySym2State p s)"
       using a2 a31 a5 assms(3) equivStatement_def trans1Symmetric by auto  
   qed
 qed
- (* have 1: "guard g a \<in> rs \<Longrightarrow>
-   \<exists>r'. equivRule (guard (applySym2Form p g) (applySym2Statement p a)) r'\<and> r' \<in> rs" for g a 
-    using assms(2) assms(3) by fastforce
-     
- (*using assms(2,3) unfolding symProtRules'_def   apply simp
-    unfolding equivForm_def equivStatement_def  apply auto*)
-  show ?case
-    apply clarify subgoal for s
-      apply (auto elim!: reachableUpToSuc)
-      subgoal for s0 g a
-        unfolding trans1Symmetric'[OF assms(3)]
-        apply (rule reachableUpTo.intros(2))
-        subgoal using Suc by auto
-        using 1 apply auto
-        using stFormSymCorrespondence1[OF assms(3)] by auto
-      done
-    done
-qed*)
 
 lemma SymLemma':
   assumes "symPredSet' N fs"
@@ -1109,7 +1128,7 @@ lemma SymLemma':
     and "p permutes {x. x \<le> N}"
     and "reachableUpTo fs rs i s"
   shows "formEval (applySym2Form p f) s"
- proof -
+proof -
   have "bij p"
     using assms(4) permutes_bij by blast
   have 0: "(inv p) permutes {x. x \<le> N}"
@@ -1173,8 +1192,8 @@ subsection \<open>More refined strengthening\<close>
 
 fun removeImplies :: "formula \<Rightarrow> formula \<Rightarrow> formula" where
 (*  "removeImplies (implyForm f1 f2) g = (if equivForm f1 g then f2 else implyForm f1 f2)"*)
-"removeImplies (implyForm f1 f2) g = 
-  (if (\<forall>s. formEval g s \<longrightarrow> formEval f1 s) then f2 else implyForm f1 f2)"
+  "removeImplies (implyForm f1 f2) g = 
+    (if (\<forall>s. formEval g s \<longrightarrow> formEval f1 s) then f2 else implyForm f1 f2)"
 | "removeImplies invf g = invf"
 
 fun strengthenForm2 :: "formula \<Rightarrow> formula \<Rightarrow> formula" where
@@ -1182,7 +1201,7 @@ fun strengthenForm2 :: "formula \<Rightarrow> formula \<Rightarrow> formula" whe
 
 fun strengthenRule2 :: "formula \<Rightarrow> rule \<Rightarrow> rule" where
   "strengthenRule2 invf (guard g a) = guard (strengthenForm2 invf g) a"
-
+declare strengthenRule2.simps [simp del]
 
 text \<open>Equivalence between strengthenRule and strengthenRule2\<close>
 
@@ -1196,7 +1215,7 @@ lemma strengthenForm2Equiv:
 
 lemma strengthenRule2Equiv:
   "equivRule (strengthenRule2 invf r) (strengthenRule invf r)"
-  apply (cases r) using strengthenForm2Equiv by auto
+  apply (cases r) using strengthenForm2Equiv strengthenRule2.simps by auto
 
 lemma equivApply2SymForm:
   assumes "p permutes {x. x \<le> N}"
@@ -1284,7 +1303,6 @@ text \<open>This corresponds to Lemma 1 in the Handbook of Model Checking
 \<close>
 lemma strengthenProtSim:
   assumes "\<And>r. r \<in> rs \<Longrightarrow> r \<in> rs' \<or> (\<exists>inv\<in>Inv. strengthenRule inv r \<in> rs')"
-(*assumes "\<forall>r. r \<in> rs \<longrightarrow> r \<in> rs' \<or> (\<exists>inv\<in>Inv. strengthenRule inv r \<in> rs')"*)
     and "\<And>i. \<forall>s. reachableUpTo I rs i s \<longrightarrow> formEval f s \<Longrightarrow>
              \<forall>s. \<forall>inv\<in>Inv. reachableUpTo I rs i s \<longrightarrow> formEval inv s"
     and "\<And>i. \<forall>s. reachableUpTo I rs' i s \<longrightarrow> formEval f s"
@@ -1335,76 +1353,63 @@ qed
 
 
 lemma strengthenProt1SimProt:
-  assumes a1:"\<forall>r. r \<in> rs \<longrightarrow>((\<exists> f . f \<in>  S \<and> strengthenRule f r \<in> rs') | r \<in> rs')" and
-  a2:"\<forall>i s f. reachableUpTo I rs' i s \<longrightarrow> f \<in> S \<longrightarrow>formEval f s" 
-shows "\<forall>s. reachableUpTo I rs i s \<longrightarrow>
-   (reachableUpTo I rs' i s \<and>(\<forall>f. f \<in> S \<longrightarrow>formEval f s))" (is "?P i")
-proof(induct_tac i)  
+  assumes a1: "\<forall>r. r \<in> rs \<longrightarrow> ((\<exists>f. f \<in> S \<and> strengthenRule f r \<in> rs') \<or> r \<in> rs')"
+    and a2: "\<forall>i s f. reachableUpTo I rs' i s \<longrightarrow> f \<in> S \<longrightarrow> formEval f s" 
+  shows "\<forall>s. reachableUpTo I rs i s \<longrightarrow>
+             (reachableUpTo I rs' i s \<and> (\<forall>f. f \<in> S \<longrightarrow> formEval f s))" (is "?P i")
+proof (induct_tac i)
   show "?P 0"
     by (meson a2 reachableSet0 reachableUpTo0)
-    
 next
   fix n
-  assume b0:"?P n"
+  assume b0: "?P n"
   show "?P (Suc n)"
-  proof((rule allI)+,(rule impI)+)
+  proof ((rule allI)+,(rule impI)+)
     fix s f
-    assume b1:"  reachableUpTo I rs (Suc n) s" 
-          
-    have " 
-        (\<exists>s0  g a.      reachableUpTo I rs n s0\<and> formEval g s0 \<and> trans1 a s0=s \<and> guard g a \<in>rs) "
+    assume b1: "reachableUpTo I rs (Suc n) s"
+    have "\<exists>s0 g a. reachableUpTo I rs n s0 \<and> formEval g s0 \<and> trans1 a s0 = s \<and> guard g a \<in> rs"
       by (metis b1 reachableUpToSuc)
-       
-    then  obtain s0   g a where c1:"     reachableUpTo I rs n s0\<and> formEval g s0 \<and>
-     trans1 a s0=s \<and> guard g a \<in>rs"
+    then obtain s0 g a where c1:
+      "reachableUpTo I rs n s0 \<and> formEval g s0 \<and> trans1 a s0 = s \<and> guard g a \<in> rs"
       by blast
     let ?r="guard g a"
-      have c2:" ((\<exists> f . f \<in>  S \<and> strengthenRule f ?r \<in> rs') | ?r \<in> rs')" 
-        using a1 c1 by blast
-      from b0 c1 c2 have c3:"\<forall>f. f \<in> S \<longrightarrow> formEval f s0"
-        by auto
-      from c2 obtain f where c2:"f \<in>  S \<and>    strengthenRule  f ?r \<in> rs' | ?r\<in> rs'"
-        by blast
-      moreover
-      {assume c2:"f \<in>  S \<and>    strengthenRule  f ?r \<in> rs'"
-      have c4:"formEval (pre (strengthenRule  f  ?r)) s0"
+    have c2:" ((\<exists> f . f \<in>  S \<and> strengthenRule f ?r \<in> rs') | ?r \<in> rs')" 
+      using a1 c1 by blast
+    from b0 c1 c2 have c3:"\<forall>f. f \<in> S \<longrightarrow> formEval f s0"
+      by auto
+    from c2 obtain f where c2:"f \<in>  S \<and>    strengthenRule  f ?r \<in> rs' | ?r\<in> rs'"
+      by blast
+    moreover
+    {
+      assume c2: "f \<in> S \<and> strengthenRule f ?r \<in> rs'"
+      have c4: "formEval (pre (strengthenRule f ?r)) s0"
         by (simp add: c1 c2 c3)  
-      have c5:"trans1 ( (act (strengthenRule  f  ?r))) s0 = trans1 (act ?r) s0"
+      have c5: "trans1 (act (strengthenRule f ?r)) s0 = trans1 (act ?r) s0"
         by simp
-         
-       
-      have c7:" reachableUpTo I rs' n s0"
-        using b0  c1 by blast
-      (*have c8:"formEval (pre (strengthenR1 Ls ss r)) s0"
-        by (metis c1 c4 evalAnd pre.simps rule.exhaust strengthenR1.simps strengthen_def) 
-        
-      have c8:"trans1  (act (strengthenR1 Ls ss r)) s0 \<in> reachableSetUpTo I rs' (Suc n)"
-        using c2 c7 c8 by auto*)
-
-      
+      have c7: "reachableUpTo I rs' n s0"
+        using b0 c1 by blast
       have "reachableUpTo I rs' (Suc n) s \<and> (\<forall>f. f \<in> S \<longrightarrow> formEval f s)"
         by (metis a2 c1 c2 c4 c7 pre.simps reachableUpTo.simps strengthenRule.simps)
-         
     }
-    {assume c2:"?r\<in> rs'"
-    have "reachableUpTo I rs' (Suc n) s \<and> (\<forall>f. f \<in> S \<longrightarrow> formEval f s)"
+    moreover
+    {
+      assume c2:"?r \<in> rs'"
+      have "reachableUpTo I rs' (Suc n) s \<and> (\<forall>f. f \<in> S \<longrightarrow> formEval f s)"
       using a2 b0 c1 c2 reachableSetNext by blast
-  }
-         
+    }
     ultimately show "reachableUpTo I rs' (Suc n) s \<and> (\<forall>f. f \<in> S \<longrightarrow> formEval f s)"
-      using \<open>f \<in> S \<and> strengthenRule f (g \<triangleright> a) \<in> rs' \<Longrightarrow> reachableUpTo I rs' (Suc n) s \<and> (\<forall>f. f \<in> S \<longrightarrow> formEval f s)\<close> by blast
-       
+      by blast
   qed
 qed 
 
 
 lemma strengthenProt2SimProt1:
-  assumes a1:"\<forall>r1. r1 \<in> rs1 \<longrightarrow>((\<exists>r f. r\<in>rs \<and>f\<in>  S \<and> r1= strengthenRule f  r 
-  \<and>  strengthenRule2 f  r \<in> rs2 ) |(  r1 \<in> rs2))" and
-  a2:"\<forall>i s f. reachableUpTo I rs2 i s\<longrightarrow> f \<in> S \<longrightarrow>formEval f s" 
-shows "\<forall>s . reachableUpTo I rs1 i s\<longrightarrow>
-   (reachableUpTo I rs2 i s\<and>(\<forall>f. f \<in> S \<longrightarrow>formEval f s))" (is "?P i")
-proof(induct_tac i)  
+  assumes a1: "\<forall>r1. r1 \<in> rs1 \<longrightarrow>
+    ((\<exists>r f. r \<in> rs \<and> f \<in> S \<and> r1 = strengthenRule f r \<and> strengthenRule2 f r \<in> rs2) \<or> r1 \<in> rs2)"
+    and a2: "\<forall>i s f. reachableUpTo I rs2 i s \<longrightarrow> f \<in> S \<longrightarrow> formEval f s" 
+  shows "\<forall>s. reachableUpTo I rs1 i s \<longrightarrow>
+          (reachableUpTo I rs2 i s \<and> (\<forall>f. f \<in> S \<longrightarrow> formEval f s))" (is "?P i")
+proof (induct_tac i)  
   show "?P 0"
     by (meson a2 reachableSet0 reachableUpTo0) 
 next
@@ -1412,99 +1417,75 @@ next
   assume b0:"?P n"
   show "?P (Suc n)"
   proof((rule allI)+,(rule impI)+)
-    fix s 
-    assume b1:" reachableUpTo I rs1 (Suc n) s"  
-    have c1:"
-        (\<exists>s0 g a. guard g a \<in>rs1 \<and>   reachableUpTo I rs1 n s0\<and> formEval g s0 \<and> trans1 a s0=s) "
+    fix s
+    assume b1: "reachableUpTo I rs1 (Suc n) s"  
+    have c1:"\<exists>s0 g a. guard g a \<in> rs1 \<and> reachableUpTo I rs1 n s0 \<and> formEval g s0 \<and> trans1 a s0 = s"
       by (metis b1 reachableUpToSuc) 
-    from c1 obtain s0 g a  where c1:"guard g a \<in>rs1 \<and>   reachableUpTo I rs1 n s0\<and> 
-      formEval g s0 \<and> trans1 a s0=s"
+    from c1 obtain s0 g a where c1:
+      "guard g a \<in> rs1 \<and> reachableUpTo I rs1 n s0 \<and> formEval g s0 \<and> trans1 a s0 = s"
+      by blast
+    have c2: "(\<exists>r f. f \<in> S \<and> r \<in> rs \<and> guard g a = strengthenRule f r \<and> strengthenRule2 f r \<in> rs2) \<or>
+              (guard g a \<in> rs2)"
+      using a1 c1 by blast
+    moreover
+    {
+      assume c2:"\<exists>r f. f \<in> S \<and> r \<in> rs \<and> guard g a = strengthenRule f r \<and> strengthenRule2 f r \<in> rs2"
+      from c2 obtain r f where c2:
+        "f \<in> S \<and> r \<in> rs \<and> guard g a = strengthenRule f r \<and> strengthenRule2 f r \<in> rs2"
         by blast
-      have c2:"(\<exists>r f. f \<in>  S \<and> r\<in>rs \<and>  (guard g a)=strengthenRule f r 
-  \<and> strengthenRule2 f r \<in> rs2)| (   (guard g a) \<in> rs2)"
-        using a1 c1 by blast
-(*" (\<exists> Ls ss. set Ls \<subseteq> set S\<and>  set ss \<subseteq> set S  \<and>  strengthenR1 Ls ss r \<in> rs') "*)
-        
-      moreover
-      {assume c2:"(\<exists>r f. f \<in>  S \<and> r\<in>rs \<and>  (guard g a)=strengthenRule f r 
-  \<and> strengthenRule2 f r \<in> rs2)"
-      from c2 obtain r f where c2:"f \<in>  S\<and> r\<in>rs \<and>  (guard g a)=strengthenRule f r 
-  \<and> strengthenRule2 f r \<in> rs2"
-        by blast
-      from b0 c1 c2 have c3:"\<forall>f. f \<in> S \<longrightarrow> formEval f s0"
+      from b0 c1 c2 have c3: "\<forall>f. f \<in> S \<longrightarrow> formEval f s0"
         by auto
-      have c4:"formEval (pre (strengthenRule2  f r)) s0"
+      have c4: "formEval (pre (strengthenRule2 f r)) s0"
         by (metis c1 c2 equivForm_def equivRule.elims(2) pre.simps strengthenRule2Equiv) 
-        
-
-      from b0 c1 c2 have c3:"\<forall>f. f \<in>S \<longrightarrow> formEval f s0"
+      from b0 c1 c2 have c3: "\<forall>f. f \<in> S \<longrightarrow> formEval f s0"
         by auto
-      have c5:"trans1 (act(strengthenRule2  f r)) s0 = trans1 (act r) s0"
+      have c5: "trans1 (act (strengthenRule2 f r)) s0 = trans1 (act r) s0"
         by (metis act.elims act.simps strengthenRule2.simps) 
-      have c6:"trans1  (act (strengthenRule2  f r)) s0 = trans1 (act r) s0"
+      have c6: "trans1 (act (strengthenRule2 f r)) s0 = trans1 (act r) s0"
         by (metis act.elims act.simps strengthenRule2.simps) 
-      have c7:" reachableUpTo I rs2 n s0"
-        using b0  c1 by blast
-      have c8:"formEval (pre (strengthenRule2 f r)) s0"
-        by (simp add: c4) 
-        
-      have c8:"reachableUpTo I rs2 (Suc n) (trans1  (act (strengthenRule2 f r)) s0)"
+      have c7: "reachableUpTo I rs2 n s0"
+        using b0 c1 by blast
+      have c8: "formEval (pre (strengthenRule2 f r)) s0"
+        by (simp add: c4)
+      have c8:"reachableUpTo I rs2 (Suc n) (trans1 (act (strengthenRule2 f r)) s0)"
         by (metis act.simps c2 c7 c8 equivRule.elims(2) pre.simps reachableSetNext strengthenRule2Equiv)
-        
-      have "reachableUpTo I rs2 (Suc n) s\<and>(\<forall>f. f \<in> S \<longrightarrow>formEval f s)"
+      have "reachableUpTo I rs2 (Suc n) s \<and> (\<forall>f. f \<in> S \<longrightarrow> formEval f s)"
         by (metis a2 act.simps c1 c2 c8 equivRule.elims(2) equivStatement_def strengthenRule2Equiv)
     }
     moreover
-    {assume c2:"(    (guard g a) \<in> rs2)"
-      have "reachableUpTo I rs2 (Suc n) s\<and>(\<forall>f. f \<in> S \<longrightarrow>formEval f s)"
+    {
+      assume c2: "guard g a \<in> rs2"
+      have "reachableUpTo I rs2 (Suc n) s \<and> (\<forall>f. f \<in> S \<longrightarrow> formEval f s)"
         using a2 b0 c1 c2 reachableSetNext by blast 
     }
-      
-    ultimately   show  "reachableUpTo I rs2 (Suc n) s\<and>(\<forall>f. f \<in> S \<longrightarrow>formEval f s)"
-        by blast
+    ultimately show "reachableUpTo I rs2 (Suc n) s \<and> (\<forall>f. f \<in> S \<longrightarrow> formEval f s)"
+      by blast
   qed
 qed 
 
 lemma strengthenProt2SimProt:
-  assumes a1:"\<forall>r. r \<in> rs \<longrightarrow>((\<exists> f. f\<in>  S \<and>  strengthenRule2 f  r \<in>rs2
-   ) |( r \<in> rs2  ))" and
-  a2:"\<forall>i s f. reachableUpTo I rs2 i s\<longrightarrow> f \<in> S \<longrightarrow>formEval f s" 
-shows "\<forall>s . reachableUpTo I rs i s\<longrightarrow>
-   (reachableUpTo I rs2 i s\<and>(\<forall>f. f \<in> S \<longrightarrow>formEval f s))" (is "?P i")
-proof(rule allI, rule impI)
+  assumes a1: "\<forall>r. r \<in> rs \<longrightarrow> ((\<exists>f. f \<in> S \<and> strengthenRule2 f r \<in> rs2) \<or> (r \<in> rs2))"
+    and a2: "\<forall>i s f. reachableUpTo I rs2 i s \<longrightarrow> f \<in> S \<longrightarrow> formEval f s" 
+  shows "\<forall>s. reachableUpTo I rs i s \<longrightarrow>
+    (reachableUpTo I rs2 i s \<and> (\<forall>f. f \<in> S \<longrightarrow> formEval f s))" (is "?P i")
+proof (rule allI, rule impI)
   fix s
-  assume b1:"reachableUpTo I rs i s"
-  let ?rs1="{r'. (\<exists>f r. f\<in>S \<and> r \<in>rs \<and> r'=strengthenRule f r\<and>strengthenRule2 f r \<in> rs2)\<or>
-            (r'\<in>rs\<and> r'\<in>rs2)}"
-  have b2:"\<forall>i s. reachableUpTo I ?rs1 i s\<longrightarrow>
- reachableUpTo I rs2 i s\<and>(\<forall>f. f \<in> S \<longrightarrow>formEval f s)" thm strengthenProt2SimProt1
-  proof(rule allI,rule_tac ?rs1.0="?rs1" and ?rs="rs" and ?rs2.0="rs2" in strengthenProt2SimProt1
-      ,auto,cut_tac a2,blast)
- qed
-
- have b3:"\<forall>s . reachableUpTo I rs i s\<longrightarrow>
- reachableUpTo I ?rs1 i s\<and>(\<forall>f. f \<in> S \<longrightarrow>formEval f s)"  thm strengthenProtSim 
- proof(rule_tac ?rs'="?rs1" and ?rs="rs"   in strengthenProt1SimProt)
-   show "\<forall>r. r \<in> rs \<longrightarrow>
-        (\<exists>f. f \<in> S \<and>
-             strengthenRule f r
-             \<in> {r'. (\<exists>f r. f \<in> S \<and> r \<in> rs \<and> r' = strengthenRule f r \<and> strengthenRule2 f r \<in> rs2) \<or>
-                    r'\<in>rs\<and> r' \<in> rs2}) \<or>
-        r \<in> {r'. (\<exists>f r. f \<in> S \<and> r \<in> rs \<and> r' = strengthenRule f r \<and> strengthenRule2 f r \<in> rs2) \<or>
-       r'\<in>rs\<and>r' \<in> rs2}"
-     using a1 by auto
- next
-   show " \<forall>i s f.
-       reachableUpTo I
-        ?rs1
-        i s \<longrightarrow>
-       f \<in> S \<longrightarrow> formEval f s"
-     using b2 by blast
- qed    
+  assume b1: "reachableUpTo I rs i s"
+  let ?rs1="{r'. (\<exists>f r. f \<in> S \<and> r \<in> rs \<and> r' = strengthenRule f r \<and> strengthenRule2 f r \<in> rs2) \<or>
+                 (r' \<in> rs \<and> r' \<in> rs2)}"
+  have b2:"\<forall>i s. reachableUpTo I ?rs1 i s \<longrightarrow>
+    reachableUpTo I rs2 i s \<and> (\<forall>f. f \<in> S \<longrightarrow> formEval f s)"
+    apply (rule allI)
+    apply (rule_tac ?rs1.0="?rs1" and ?rs="rs" and ?rs2.0="rs2" in strengthenProt2SimProt1)
+    apply auto apply (cut_tac a2) by blast
+  have b3: "\<forall>s. reachableUpTo I rs i s\<longrightarrow>
+    reachableUpTo I ?rs1 i s \<and> (\<forall>f. f \<in> S \<longrightarrow> formEval f s)"
+    apply (rule strengthenProt1SimProt)
+    using a1 apply auto[1]
+    using b2 by blast
   show "reachableUpTo I rs2 i s \<and> (\<forall>f. f \<in> S \<longrightarrow> formEval f s)"
     using b1 b2 b3 by blast
-    
- qed
+qed
  
 subsection \<open>Abstraction\<close>
 
@@ -2206,25 +2187,25 @@ primrec varOfExp :: "expType \<Rightarrow> varType set" and
   where
   "varOfExp  (IVar v)  = varsOfVar v" |
   "varOfExp  (Const j) = set []" |
-  "varOfExp  (iteForm f e1 e2) = varOfForm f \<union> varOfExp e1 \<union> varOfExp  e2" |
-  "varOfExp  dontCareExp={}"|
-  "varOfForm (eqn e1 e2) = varOfExp e1 \<union> varOfExp  e2" |
+  "varOfExp  (iteForm f e1 e2) = varOfForm f \<union> varOfExp e1 \<union> varOfExp e2" |
+  "varOfExp  dontCareExp = {}"|
+  "varOfForm (eqn e1 e2) = varOfExp e1 \<union> varOfExp e2" |
   "varOfForm (andForm f1 f2) = varOfForm f1 \<union> varOfForm f2" |
   "varOfForm (neg f1) = varOfForm f1" |
   "varOfForm (orForm f1 f2) = varOfForm f1 \<union> varOfForm f2" |
   "varOfForm (implyForm f1 f2) = varOfForm f1 \<union> varOfForm f2" |
   "varOfForm (chaos) = {}"|
   "varOfForm (forallForm pf N) = \<Union>{S. \<exists>i. i \<le> N \<and> S = varOfForm (pf i)}"|
-  "varOfForm dontCareForm={}" |
-  "varOfForm (forallFormExcl pf j N) = \<Union>{S. \<exists>i. j\<noteq>i\<and>i \<le> N \<and> S = varOfForm (pf i)}"
+  "varOfForm dontCareForm = {}" |
+  "varOfForm (forallFormExcl pf j N) = \<Union>{S. \<exists>i. j \<noteq> i \<and> i \<le> N \<and> S = varOfForm (pf i)}"
 
 primrec constOfExp :: "expType \<Rightarrow> scalrValueType set" and
   constOfForm :: "formula \<Rightarrow> scalrValueType set"
   where
   "constOfExp  (IVar v)  = {}" |
   "constOfExp  (Const j) = set [j]" |
-  "constOfExp  (iteForm f e1 e2) = constOfForm f \<union> constOfExp e1 \<union> constOfExp  e2" |
-  "constOfExp  dontCareExp={}"|
+  "constOfExp  (iteForm f e1 e2) = constOfForm f \<union> constOfExp e1 \<union> constOfExp e2" |
+  "constOfExp  dontCareExp = {}"|
   "constOfForm (eqn e1 e2) = constOfExp e1 \<union> constOfExp  e2" |
   "constOfForm (andForm f1 f2) = constOfForm f1 \<union> constOfForm f2" |
   "constOfForm (neg f1) = constOfForm f1" |
@@ -2232,111 +2213,57 @@ primrec constOfExp :: "expType \<Rightarrow> scalrValueType set" and
   "constOfForm (implyForm f1 f2) = constOfForm f1 \<union> constOfForm f2" |
   "constOfForm (chaos) = {}"|
   "constOfForm (forallForm pf N) = \<Union>{S. \<exists>i. i \<le> N \<and> S = constOfForm (pf i)}"|
-  "constOfForm dontCareForm={}" |
-  "constOfForm (forallFormExcl pf j N) = \<Union>{S. \<exists>i. j\<noteq>i\<and>i \<le> N \<and> S = constOfForm (pf i)}"
+  "constOfForm dontCareForm = {}" |
+  "constOfForm (forallFormExcl pf j N) = \<Union>{S. \<exists>i. j \<noteq> i \<and> i \<le> N \<and> S = constOfForm (pf i)}"
 
 definition safeIndexExp::"nat\<Rightarrow>expType\<Rightarrow>bool" where [simp]:
-"safeIndexExp M e \<equiv> \<forall>c n. c\<in>constOfExp e \<longrightarrow> \<not>(c = index n\<and> M<n)"
+  "safeIndexExp M e \<equiv> \<forall>c n. c \<in> constOfExp e \<longrightarrow> \<not>(c = index n \<and> M < n)"
 
 definition safeIndexForm::"nat\<Rightarrow>formula\<Rightarrow>bool" where [simp]:
-"safeIndexForm M f \<equiv> \<forall>c n. c\<in>constOfForm f \<longrightarrow> \<not>(c = index n\<and> M<n)"
- 
-lemma dontAffect:
-  shows a1:"((\<forall>v. v\<in>varOfExp e\<longrightarrow> (s v= s' v))\<longrightarrow>expEval e s = expEval e s')\<and>
-  ((\<forall>v. v\<in>varOfForm f\<longrightarrow> (s v= s' v))\<longrightarrow>formEval f s = formEval f s')" 
-  (is "( (\<forall>v. ?P v e s s' )\<longrightarrow>?P2 e s s') \<and> ((\<forall>v. ?Q v f  s s'  )\<longrightarrow>?Q2 f s s')") 
-proof(induction rule: expType_formula.induct,force,force,force,force,force,force,force,force,force)
-(*proof(induct_tac e and f,force,force,force,force,force,force,force,force,force )*)
-  next
-    case (forallForm x1 x2)
-    show ?case
-      using forallForm.IH by auto
-  next
-    case chaos
-    show ?case
-      by auto
-  next
-    case  (forallFormExcl x1 x2 x3)
-    show ?case
-      using forallFormExcl.IH rangeI by fastforce
-  qed( auto)
- 
+  "safeIndexForm M f \<equiv> \<forall>c n. c \<in> constOfForm f \<longrightarrow> \<not>(c = index n \<and> M < n)"
 
-(*a1:"(((\<forall> v. v\<in> varOfExp e \<longrightarrow>v\<noteq>dontCareVar\<and> (v = absTransfVar M v ))\<and>safeIndexExp M e \<and> e\<noteq>dontCareExp)
-        \<longrightarrow> e\<noteq>dontCareExp\<and>e = absTransfExp M e)\<and> 
-  (((\<forall> v. v\<in> varOfForm f \<longrightarrow> v\<noteq>dontCareVar\<and>(v = absTransfVar M v )) \<and> safeIndexForm M f \<and>f\<noteq>dontCareForm)
-  \<longrightarrow>f\<noteq>dontCareForm\<and> f = absTransfForm M f )  "
-(is "?Pe e \<and> ?Pf f")
-(* proof(induction rule: expType_formula.induct) *)
-proof(induct_tac e and f,force,case_tac x,force,force,force,force )
-  fix f e1 e2 
-  assume b1:"?Pf f" and
-  b2:"?Pe e1" and b3:"?Pe e2"
-  show "?Pe (iteForm f e1 e2 )"
-  proof(rule impI)
-    assume c0:"(\<forall>v. v \<in> varOfExp (iteForm f e1 e2) \<longrightarrow> v \<noteq> dontCareVar \<and> v = absTransfVar M v) \<and>
-    safeIndexExp M (iteForm f e1 e2)"
-    have c1:"((\<forall> v. v\<in> varOfExp e1 \<longrightarrow>v\<noteq>dontCareVar\<and> (v = absTransfVar M v ))\<and>safeIndexExp M e1
-       \<and> e1\<noteq>dontCareExp)"
-      by(cut_tac c0, simp)
-    have c2:"((\<forall> v. v\<in> varOfExp e2 \<longrightarrow>v\<noteq>dontCareVar\<and> (v = absTransfVar M v ))\<and>safeIndexExp M e2)"
-      by(cut_tac c0, simp)
-    have c3:"((\<forall> v. v\<in> varOfForm f \<longrightarrow> v\<noteq>dontCareVar\<and>(v = absTransfVar M v )) \<and> safeIndexForm M f)"
-      by(cut_tac c0, simp)
-    have c4:" e1 = absTransfExp M e1"
-      using b2 c1 by blast
-    have c5:" e2 = absTransfExp M e2"
-      using b3 c2 by blast  
-     have c6:" f = absTransfForm M f"
-       using b1 c3 by blast
-     show "iteForm f e1 e2 = absTransfExp M (iteForm f e1 e2) "
-      
-  case (IVar x)
+lemma dontAffect:
+  "((\<forall>v. v \<in> varOfExp e \<longrightarrow> s v = s' v) \<longrightarrow> expEval e s = expEval e s') \<and>
+   ((\<forall>v. v \<in> varOfForm f \<longrightarrow> s v = s' v) \<longrightarrow> formEval f s = formEval f s')" 
+proof (induction rule: expType_formula.induct)
+  case (forallForm x1 x2)
   show ?case
-*)  
+    using forallForm.IH by auto
+next
+  case (forallFormExcl x1 x2 x3)
+  show ?case
+    using forallFormExcl.IH rangeI by fastforce
+qed (auto)
+
 lemma absDontAffect:
-  assumes  
-  a2:"(\<forall>v. v\<in>varOfForm f\<longrightarrow> (s v= (abs1 M s) v))"
+  assumes "\<forall>v. v \<in> varOfForm f \<longrightarrow> s v = abs1 M s v"
   shows "formEval f s = formEval f (abs1 M s)"
-  by (simp add: a2 dontAffect)
-   
+  by (simp add: assms dontAffect)
 
 lemma strengthenRule2Keep:
-  assumes     a2:" wellFormedRule N r"
+  assumes "wellFormedRule N r"
   shows "wellFormedRule N (strengthenRule2 f r)"
   by (metis assms strengthenRule2.simps wellFormedRule.elims(2) wellFormedRule.simps)  
 
 
-definition symRules :: "nat \<Rightarrow> (rule set) \<Rightarrow> bool" where
-  "symRules N rs =
-    (\<forall>r p. r\<in>rs \<longrightarrow>p permutes {x. x \<le> N}  \<longrightarrow> (\<exists>r'. r'\<in>rs\<and> equivRule (applySym2Rule p r ) r'))"
-
-(*lemma symStrengthenRule2:
-  assumes a1:"symProtRules N rs" and
-  a2:"symPredSet N fs"
-shows "symProtRules N {r'. (EX  r f. f \<in>fs \<and> r\<in>rs \<and> r'=strengthenRule2 f r) |r'\<in> rs}"
-*)  
-
-
-    
-definition oneParamCons::"nat \<Rightarrow>(nat => rule) => rule set" where [simp]:
-"oneParamCons N pr \<equiv>{r. \<exists>i. i\<le> N \<and> r = pr i}"
+definition oneParamCons :: "nat \<Rightarrow> (nat \<Rightarrow> rule) \<Rightarrow> rule set" where [simp]:
+  "oneParamCons N pr \<equiv> {r. \<exists>i. i \<le> N \<and> r = pr i}"
 
 lemma symParaRuleInfSymRuleSet:
-  assumes a:"symParamRule N pr"
+  assumes a: "symParamRule N pr"
   shows "symProtRules' N (oneParamCons N pr)"
-proof(unfold symProtRules'_def,(rule allI)+,rule)
+proof (unfold symProtRules'_def,(rule allI)+,rule)
   fix p r
-  assume a1:" p permutes {x. x \<le> N} \<and> r \<in> oneParamCons N pr"
-  from a1 have a2:"\<exists>i. i\<le> N \<and> r = pr i"
-    by(unfold oneParamCons_def,auto)
-  then obtain i where a3:"i\<le>N \<and> r=pr i"
+  assume a1: "p permutes {x. x \<le> N} \<and> r \<in> oneParamCons N pr"
+  from a1 have a2: "\<exists>i. i \<le> N \<and> r = pr i"
+    by (unfold oneParamCons_def, auto)
+  then obtain i where a3: "i \<le> N \<and> r = pr i"
     by blast
-  have a4:"p i \<le>N"
+  have a4: "p i \<le> N"
     using a3 local.a1 permutes_in_image by fastforce 
-  show " \<exists>r'. r' \<in> oneParamCons N pr \<and> equivRule (applySym2Rule p r) r'"
-    apply(cut_tac a a1 a3, unfold  symParamRule_def)
-    apply(rule_tac x="pr (p i)" in exI)
+  show "\<exists>r'. r' \<in> oneParamCons N pr \<and> equivRule (applySym2Rule p r) r'"
+    apply (cut_tac a a1 a3, unfold symParamRule_def)
+    apply (rule_tac x="pr (p i)" in exI)
     apply auto
     using a4 oneParamCons_def by auto
 qed
@@ -2346,46 +2273,46 @@ theorem symProtRulesUnion:
   shows "symProtRules' N (A \<union> B)"
   by (metis UnCI UnE a2 local.a1 symProtRules'_def)
 
-definition oneParamFormCons::"nat \<Rightarrow>(nat => formula) => formula set" where
-"oneParamFormCons N pr \<equiv>{r. \<exists>i. i\<le> N \<and> r = pr i}"
+definition oneParamFormCons::"nat \<Rightarrow>(nat \<Rightarrow> formula) \<Rightarrow> formula set" where
+  "oneParamFormCons N pr \<equiv> {r. \<exists>i. i \<le> N \<and> r = pr i}"
 
-definition oneParamFormCons2::"nat \<Rightarrow>(nat =>nat\<Rightarrow> formula) => formula set" where
-"oneParamFormCons2 N pr \<equiv>{r. \<exists>i j. i\<le> N \<and> j\<le>N \<and>r = pr i j}"
+definition oneParamFormCons2::"nat \<Rightarrow> (nat \<Rightarrow> nat \<Rightarrow> formula) \<Rightarrow> formula set" where
+  "oneParamFormCons2 N pr \<equiv> {r. \<exists>i j. i \<le> N \<and> j \<le> N \<and> r = pr i j}"
 
 lemma symParaFormInfSymFormSet:
   assumes a:"symParamForm N pr"
   shows "symPredSet' N (oneParamFormCons N pr)"
-proof(unfold symPredSet'_def,(rule allI)+,rule)
+proof (unfold symPredSet'_def,(rule allI)+,rule)
   fix p r
-  assume a1:" p permutes {x. x \<le> N} \<and> r \<in> oneParamFormCons N pr"
-  from a1 have a2:"\<exists>i. i\<le> N \<and> r = pr i"
-    by(unfold oneParamFormCons_def,auto)
-  then obtain i where a3:"i\<le>N \<and> r=pr i"
+  assume a1: "p permutes {x. x \<le> N} \<and> r \<in> oneParamFormCons N pr"
+  from a1 have a2: "\<exists>i. i \<le> N \<and> r = pr i"
+    by (unfold oneParamFormCons_def,auto)
+  then obtain i where a3: "i \<le> N \<and> r = pr i"
     by blast
-  have a4:"p i \<le>N"
+  have a4:"p i \<le> N"
     using a3 local.a1 permutes_in_image by fastforce 
-  show " \<exists>r'. r' \<in> oneParamFormCons N pr \<and> equivForm (applySym2Form p r) r'"
-    apply(cut_tac a a1 a3, unfold  symParamForm_def)
-    apply(rule_tac x="pr (p i)" in exI)
+  show "\<exists>r'. r' \<in> oneParamFormCons N pr \<and> equivForm (applySym2Form p r) r'"
+    apply (cut_tac a a1 a3, unfold symParamForm_def)
+    apply (rule_tac x="pr (p i)" in exI)
     apply auto
     using a4 oneParamFormCons_def by auto
 qed
 
 lemma symParaFormInfSymFormSet2:
-  assumes a:"symParamForm2 N pr"
+  assumes a: "symParamForm2 N pr"
   shows "symPredSet' N (oneParamFormCons2 N pr)"
-proof(unfold symPredSet'_def,(rule allI)+,rule)
+proof (unfold symPredSet'_def,(rule allI)+,rule)
   fix p r
-  assume a1:" p permutes {x. x \<le> N} \<and> r \<in> oneParamFormCons2 N pr"
-  from a1 have a2:"\<exists>i j. i\<le> N \<and> j\<le> N \<and>r = pr i j"
-    by(unfold oneParamFormCons2_def,auto)
-  then obtain i j where a3:"i\<le>N  \<and> j\<le> N\<and> r=pr i j"
+  assume a1: "p permutes {x. x \<le> N} \<and> r \<in> oneParamFormCons2 N pr"
+  from a1 have a2: "\<exists>i j. i \<le> N \<and> j \<le> N \<and> r = pr i j"
+    by (unfold oneParamFormCons2_def,auto)
+  then obtain i j where a3: "i \<le> N \<and> j \<le> N \<and> r = pr i j"
     by blast
-  have a4:"p i \<le>N \<and> p j \<le>N"
+  have a4:"p i \<le> N \<and> p j \<le> N"
     using a3 local.a1 permutes_in_image by fastforce 
-  show " \<exists>r'. r' \<in> oneParamFormCons2 N pr \<and> equivForm (applySym2Form p r) r'"
-    apply(cut_tac a a1 a3, unfold  symParamForm2_def)
-    apply(rule_tac x="pr (p i) (p j)" in exI) 
+  show "\<exists>r'. r' \<in> oneParamFormCons2 N pr \<and> equivForm (applySym2Form p r) r'"
+    apply (cut_tac a a1 a3, unfold  symParamForm2_def)
+    apply (rule_tac x="pr (p i) (p j)" in exI) 
     apply auto
     using a4 oneParamFormCons2_def by auto
 qed
@@ -2395,20 +2322,19 @@ theorem symPredsUnion:
   shows "symPredSet' N (A \<union> B)"
   using a2 local.a1 by fastforce 
 
-definition constrInv::"((nat\<Rightarrow>formula)\<times>(nat\<Rightarrow>formula))=>nat=> nat=>formula" where [simp]:
-"constrInv pair i j\<equiv>(((fst pair)  i)\<longrightarrow>\<^sub>f (neg (  (Const (index i)) =\<^sub>f (Const (index j))))\<longrightarrow>\<^sub>f((snd pair) j))"
+definition constrInv :: "((nat \<Rightarrow> formula) \<times> (nat \<Rightarrow> formula)) \<Rightarrow> nat \<Rightarrow> nat \<Rightarrow> formula" where [simp]:
+  "constrInv pair i j \<equiv> fst pair i \<longrightarrow>\<^sub>f \<not>\<^sub>f Const (index i) =\<^sub>f Const (index j) \<longrightarrow>\<^sub>f snd pair j"
 
-definition constrInvByExcl::"((nat\<Rightarrow>formula)\<times>(nat\<Rightarrow>formula))=>nat=> nat\<Rightarrow>formula" where [simp]:
-"constrInvByExcl pair i  N\<equiv>(((fst pair)  i)\<longrightarrow>\<^sub>f  forallFormExcl (snd pair) i N)"
+definition constrInvByExcl :: "((nat \<Rightarrow> formula) \<times> (nat \<Rightarrow> formula)) \<Rightarrow> nat \<Rightarrow> nat \<Rightarrow> formula" where
+  "constrInvByExcl pair i N \<equiv> fst pair i \<longrightarrow>\<^sub>f forallFormExcl (snd pair) i N"
 
-definition constrInvByExcls::"((nat\<Rightarrow>formula)\<times>(nat\<Rightarrow>formula)) set=>nat\<Rightarrow>formula set" where [simp]:
-"constrInvByExcls pairs   N\<equiv>
-  {f. \<exists>i pair. pair\<in>pairs\<and> i\<le>N\<and>f=(((fst pair)  i)\<longrightarrow>\<^sub>f  forallFormExcl (snd pair) i N)}"
+definition constrInvByExcls :: "((nat \<Rightarrow> formula) \<times> (nat \<Rightarrow> formula)) set \<Rightarrow> nat \<Rightarrow> formula set" where [simp]:
+  "constrInvByExcls pairs N \<equiv>
+    {f. \<exists>i pair. pair \<in> pairs \<and> i \<le> N \<and> f = (fst pair i \<longrightarrow>\<^sub>f forallFormExcl (snd pair) i N)}"
 
-definition symPair::"((nat\<Rightarrow>formula)\<times>(nat\<Rightarrow>formula)) \<Rightarrow>nat\<Rightarrow>bool" where [simp]:
-"symPair x N\<equiv>(symParamForm N (fst x)) & (symParamForm N (snd x))"
+definition symPair :: "((nat \<Rightarrow> formula) \<times> (nat \<Rightarrow> formula)) \<Rightarrow> nat \<Rightarrow> bool" where [simp]:
+  "symPair x N \<equiv> symParamForm N (fst x) \<and> symParamForm N (snd x)"
 
- 
 lemma permute_ij:
   fixes N i j :: nat
   assumes "1 \<le> N" "i \<le> N" "j \<le> N" "i \<noteq> j"
@@ -2458,309 +2384,273 @@ proof -
   let ?p="inv p"
   have "?p permutes {i. i \<le> N}"
     using local.a1 permutes_inv by blast
-    
   show "\<exists>p. p permutes {i. i \<le> N} \<and> p 0 = i \<and> p 1 = j"
     by (metis \<open>inv p permutes {i. i \<le> N}\<close> local.a1 permutes_inverses(2))
-qed    
+qed
     
 lemma symOnFunc:
-  assumes a1:"symPair pair  N"  and a2:"1\<le>N"
-  shows "\<forall>i j. i\<le>N \<longrightarrow> j\<le>N \<longrightarrow>i\<noteq>j\<longrightarrow>
-  (\<exists>p. p permutes {i. i \<le> N}\<and> equivForm (applySym2Form p (constrInv pair i j)) (constrInv pair 0 1) )"
-proof((rule allI)+,(rule impI)+)
+  assumes a1: "symPair pair N"
+    and a2: "1 \<le> N"
+  shows "\<forall>i j. i \<le> N \<longrightarrow> j \<le> N \<longrightarrow> i \<noteq> j\<longrightarrow>
+    (\<exists>p. p permutes {i. i \<le> N} \<and> equivForm (applySym2Form p (constrInv pair i j)) (constrInv pair 0 1))"
+proof ((rule allI)+,(rule impI)+)
   fix i j
-  assume "i\<le>N" and "j\<le>N" and "i\<noteq>j"
+  assume "i \<le> N" and "j \<le> N" and "i \<noteq> j"
   have "\<exists>p. p permutes {i. i \<le> N} \<and> p i = 0 \<and> p j = 1"
     using \<open>i \<le> N\<close> \<open>i \<noteq> j\<close> \<open>j \<le> N\<close> a2 permute_ij by blast
-  then obtain p where b1:"p permutes {i. i \<le> N} \<and> p i = 0 \<and> p j = 1"
+  then obtain p where b1: "p permutes {i. i \<le> N} \<and> p i = 0 \<and> p j = 1"
     by blast
-  show " \<exists>p. p permutes {i. i \<le> N} \<and> equivForm (applySym2Form p (constrInv pair i j)) (constrInv pair 0 1)"
-  proof(rule_tac x="p" in exI)
+  show "\<exists>p. p permutes {i. i \<le> N} \<and> equivForm (applySym2Form p (constrInv pair i j)) (constrInv pair 0 1)"
+  proof (rule_tac x="p" in exI)
     show "p permutes {i. i \<le> N} \<and> equivForm (applySym2Form p (constrInv pair i j)) (constrInv pair 0 1)"
-    proof(cut_tac a1, rule conjI)
-      show " p permutes {i. i \<le> N}"
+    proof (cut_tac a1, rule conjI)
+      show "p permutes {i. i \<le> N}"
         using \<open>p permutes {i. i \<le> N} \<and> p i = 0 \<and> p j = 1\<close> by blast
     next
-      have c1:"equivForm  (applySym2Form p (fst pair i)) (fst pair 0)"
+      have c1:"equivForm (applySym2Form p (fst pair i)) (fst pair 0)"
         using \<open>i \<le> N\<close> b1 local.a1 mem_Collect_eq symParamForm_def by fastforce
-      have c2:"equivForm  (applySym2Form p (snd pair j)) (snd pair 1)"
-         using \<open>j \<le> N\<close> b1 local.a1 mem_Collect_eq symParamForm_def by fastforce
-       show "equivForm (applySym2Form p (constrInv pair i j))  (constrInv pair 0 1)"
-        apply( unfold constrInv_def,simp)
-        apply(cut_tac c1 c2, unfold equivForm_def,auto )
-         using b1 by linarith
-     qed
-   qed
- qed
+      have c2:"equivForm (applySym2Form p (snd pair j)) (snd pair 1)"
+        using \<open>j \<le> N\<close> b1 local.a1 mem_Collect_eq symParamForm_def by fastforce
+      show "equivForm (applySym2Form p (constrInv pair i j)) (constrInv pair 0 1)"
+        apply (unfold constrInv_def,simp)
+        apply(cut_tac c1 c2, unfold equivForm_def,auto)
+        using b1 by linarith
+    qed
+  qed
+qed
 
 lemma symOnFuncInv:
-  assumes a1:"symPair pair  N"  and a2:"1\<le>N"
-  shows "\<forall>i j. i\<le>N \<longrightarrow> j\<le>N \<longrightarrow>i\<noteq>j\<longrightarrow>
-  (\<exists>p. p permutes {i. i \<le> N}\<and> 
-  equivForm (applySym2Form p (constrInv pair 0 1)) (constrInv pair i j) )"
-proof((rule allI)+,(rule impI)+)
+  assumes a1: "symPair pair N"
+    and a2:"1\<le>N"
+  shows "\<forall>i j. i \<le> N \<longrightarrow> j \<le> N \<longrightarrow> i \<noteq> j \<longrightarrow>
+    (\<exists>p. p permutes {i. i \<le> N} \<and> 
+         equivForm (applySym2Form p (constrInv pair 0 1)) (constrInv pair i j))"
+proof ((rule allI)+,(rule impI)+)
   fix i j
-  assume "i\<le>N" and "j\<le>N" and "i\<noteq>j"
+  assume "i \<le> N" and "j \<le> N" and "i \<noteq> j"
   have "\<exists>p. p permutes {i. i \<le> N} \<and> p 0 = i \<and> p 1 = j"
     using \<open>i \<le> N\<close> \<open>i \<noteq> j\<close> \<open>j \<le> N\<close> a2 permute_inv_ij by blast
-  then obtain p where b1:"p permutes {i. i \<le> N} \<and> p 0 = i \<and> p 1 = j"
+  then obtain p where b1: "p permutes {i. i \<le> N} \<and> p 0 = i \<and> p 1 = j"
     by blast
-  show " \<exists>p. p permutes {i. i \<le> N} \<and>
-   equivForm (applySym2Form p (constrInv pair 0 1 )) (constrInv pair i j)"
-  proof(rule_tac x="p" in exI)
-    show "p permutes {i. i \<le> N} \<and> equivForm (applySym2Form p (constrInv pair  0 1)) (constrInv pair i j)"
+  show "\<exists>p. p permutes {i. i \<le> N} \<and> equivForm (applySym2Form p (constrInv pair 0 1)) (constrInv pair i j)"
+  proof (rule_tac x=p in exI)
+    show "p permutes {i. i \<le> N} \<and> equivForm (applySym2Form p (constrInv pair 0 1)) (constrInv pair i j)"
     proof(cut_tac a1, rule conjI)
-      show " p permutes {i. i \<le> N}"
-        using \<open>p permutes {i. i \<le> N} \<and> p 0 = i \<and> p 1= j\<close> by blast
+      show "p permutes {i. i \<le> N}"
+        using \<open>p permutes {i. i \<le> N} \<and> p 0 = i \<and> p 1 = j\<close> by blast
     next
-      have c1:"equivForm  (applySym2Form p (fst pair 0)) (fst pair i)"
+      have c1: "equivForm (applySym2Form p (fst pair 0)) (fst pair i)"
         using \<open>i \<le> N\<close> b1 local.a1 mem_Collect_eq symParamForm_def by fastforce
-      have c2:"equivForm  (applySym2Form p (snd pair 1)) (snd pair j)"
-         using \<open>j \<le> N\<close> a2 b1 local.a1  symParamForm_def by fastforce
-       show "equivForm (applySym2Form p (constrInv pair 0 1))  (constrInv pair i j)"
-        apply( unfold constrInv_def,simp)
-        apply(cut_tac c1 c2, unfold equivForm_def,auto )
-
+      have c2: "equivForm (applySym2Form p (snd pair 1)) (snd pair j)"
+         using \<open>j \<le> N\<close> a2 b1 local.a1 symParamForm_def by fastforce
+      show "equivForm (applySym2Form p (constrInv pair 0 1)) (constrInv pair i j)"
+        apply (unfold constrInv_def,simp)
+         apply (cut_tac c1 c2, unfold equivForm_def,auto)
          using One_nat_def b1 apply presburger
          using \<open>i \<noteq> j\<close> by blast
-     qed
-   qed
- qed
+    qed
+  qed
+qed
 
 
 lemma strengthensymPair:
-  assumes a1:"symPair  p N" and "symParamRule N r"
-  shows "symParamRule N  (%i. (strengthenRule2  (constrInvByExcl p i N) (r i)))"
-proof(rule symParamStrengthenRule2)
+  assumes a1: "symPair p N"
+    and "symParamRule N r"
+  shows "symParamRule N (\<lambda>i. strengthenRule2 (constrInvByExcl p i N) (r i))"
+proof (rule symParamStrengthenRule2)
   show "symParamRule N r"
     using assms(2) by auto
 next
-  have "symParamForm N (\<lambda>i . forallFormExcl (snd p) i N)"
-    apply(rule symParamFormForallExcl)
+  have "symParamForm N (\<lambda>i. forallFormExcl (snd p) i N)"
+    apply (rule symParamFormForallExcl)
     using local.a1 symPair_def symParamForm2_def symParamForm_def by blast
-    
-  show "symParamForm N (\<lambda>i. constrInvByExcl p i N) "   thm symParamFormForallExcl
-    apply(simp only:constrInvByExcl_def)
-    apply(rule symParamFormImply)
+  show "symParamForm N (\<lambda>i. constrInvByExcl p i N)"
+    apply (simp only: constrInvByExcl_def)
+    apply (rule symParamFormImply)
     using local.a1 symPair_def apply blast
     by (simp add: \<open>symParamForm N (\<lambda>i. forallFormExcl (snd p) i N)\<close>)
-qed    
+qed
 
 lemma symParamUN:
-  assumes a1:"\<And>s. s\<in>S \<longrightarrow> symProtRules' N s"
-  shows " symProtRules' N (\<Union>S)"
+  assumes a1: "\<And>s. s\<in>S \<longrightarrow> symProtRules' N s"
+  shows "symProtRules' N (\<Union>S)"
   using local.a1 by fastforce
-  
+
 lemma SymLemmaOnExcl:
   assumes "symPredSet' N Is"
     and "symProtRules' N rs"
     and "1 \<le> N"
-    and "symPair   pair N"
+    and "symPair pair N"
     and "reachableUpTo Is rs k s"
-    and "\<forall>s i.  reachableUpTo Is rs i s \<longrightarrow> formEval ( constrInv pair 0 1 )  s"
+    and "\<forall>s i. reachableUpTo Is rs i s \<longrightarrow> formEval (constrInv pair 0 1) s"
     and "i\<le>N"
-  shows   " 
-     formEval ( constrInvByExcl pair i  N)   s  "
-
-proof(simp,rule+)
+  shows "formEval (constrInvByExcl pair i N) s"
+proof (simp add: constrInvByExcl_def, rule+)
   fix j
-  assume b1:"formEval (fst pair i) s " and
-  b2:"  j \<noteq> i" and b3:"j \<le> N "
-  have c1:"(\<exists>p. p permutes {i. i \<le> N}\<and> 
-    equivForm (applySym2Form p (constrInv pair 0 1)) (constrInv pair i j) )"
-    using assms(3) assms(4) assms(7) b2 b3 symOnFuncInv by blast
-  then obtain p where c1:"p permutes {i. i \<le> N}\<and> 
+  assume b1: "formEval (fst pair i) s" and b2: "j \<noteq> i" and b3: "j \<le> N"
+  have c1: "\<exists>p. p permutes {i. i \<le> N} \<and>
+    equivForm (applySym2Form p (constrInv pair 0 1)) (constrInv pair i j)"
+    using assms(3,4,7) b2 b3 symOnFuncInv by blast
+  then obtain p where c1: "p permutes {i. i \<le> N} \<and>
     equivForm (applySym2Form p (constrInv pair 0 1)) (constrInv pair i j)" 
     by blast
-  have c2:"formEval (applySym2Form p (constrInv pair 0 1)) s"
-    using SymLemma' assms(1) assms(2) assms(5) assms(6) c1 by blast
-  have c3:"formEval (constrInv pair i j) s"
+  have c2: "formEval (applySym2Form p (constrInv pair 0 1)) s"
+    using SymLemma' assms(1,2,5,6) c1 by blast
+  have c3: "formEval (constrInv pair i j) s"
     using c1 c2 equivForm_def by blast
-    
   show "formEval (snd pair j) s"
-    by(cut_tac b1 b2 c3, unfold constrInv_def,auto)
+    by (cut_tac b1 b2 c3, unfold constrInv_def,auto)
 qed
 
 
-primrec getValueType::"scalrValueType\<Rightarrow>string" where [simp]:
-" getValueType (enum t v) =''enum''"|
-" getValueType (index n) =''nat''"|
-"  getValueType (boolV n) =''bool''"|
-"  getValueType (dontCare) =''any''"
+primrec getValueType :: "scalrValueType \<Rightarrow> string" where [simp]:
+  "getValueType (enum t v) = ''enum''"|
+  "getValueType (index n) = ''nat''"|
+  "getValueType (boolV n) = ''bool''"|
+  "getValueType (dontCare) =''any''"
 
 
-definition typeOf::"state \<Rightarrow>varType \<Rightarrow>string " where [simp]:
-"typeOf s x =
-   getValueType (s x)" 
+definition typeOf :: "state \<Rightarrow> varType \<Rightarrow> string" where [simp]:
+  "typeOf s x = getValueType (s x)" 
 
-definition isBoolVal::"state \<Rightarrow> varType \<Rightarrow> bool" where [simp]:
-"isBoolVal s e\<equiv>typeOf s e =''bool'' "
+definition isBoolVal :: "state \<Rightarrow> varType \<Rightarrow> bool" where [simp]:
+  "isBoolVal s e \<equiv> typeOf s e = ''bool''"
 
-definition isEnumVal::"state \<Rightarrow>varType \<Rightarrow> bool" where [simp]:
-"isEnumVal s e\<equiv>typeOf s e =''enum'' "
+definition isEnumVal :: "state \<Rightarrow> varType \<Rightarrow> bool" where [simp]:
+  "isEnumVal s e \<equiv> typeOf s e = ''enum''"
 
 lemma enumValAbsRemainSame:
-  assumes a:"isEnumVal s  x " and b:" absTransfVar M x =x" and c:"x\<noteq>dontCareVar"
-  shows "s x=absTransfConst  M (s x)"
-  apply(cut_tac a b,case_tac x, case_tac "s (Ident x1)",simp,simp,simp,simp)
-  apply(case_tac "(s (Para x21 x22))" )
-      apply (simp add: abs1Eq)
-     apply (simp add: abs1Eq)
-    apply (simp add: abs1Eq)
-   apply (simp add: abs1Eq)
-  apply(cut_tac c,simp )
-  done
+  assumes a: "isEnumVal s x"
+    and b: "absTransfVar M x = x"
+    and c: "x \<noteq> dontCareVar"
+  shows "s x = absTransfConst M (s x)"
+  apply (cut_tac a b,case_tac x, case_tac "s (Ident x1)";simp)
+   apply (case_tac "s (Para x21 x22)")
+  using c by (auto simp add: abs1Eq)
 
 lemma CMP:
-  assumes a1:"\<And>r. r\<in>rs \<longrightarrow> wellFormedRule N r"
-    and (*a2:"(F N) \<subseteq>{f'. \<exists>p f. f \<in>(F M) \<and> p permutes {i. i \<le> N}& equivForm f' (applySym2Form p f)}"*)
-    a2:"\<forall>f. f\<in>F \<longrightarrow> symPair f N "
-    and a3:"symProtRules' N rs" 
-    and a4:"symPredSet' N Is"
-    and a5:"M\<le>N"
-   (* and a6:"\<forall>N. symPredSet' N (F N)"*)
-   (* and a7:"\<forall>i f s. f\<in>(F M) \<longrightarrow> reachableUpTo ({f'. \<exists>f. f \<in>Is \<and> f'=absTransfForm M f}) 
-   {r'. \<exists>r. r \<in>rs2 \<and> r'=absTransfRule M r} i s \<longrightarrow> formEval f s"*)
-    and a7:"\<forall>i f s. f\<in>F  \<longrightarrow> reachableUpTo ({f'. \<exists>f. f \<in>Is \<and> f'=absTransfForm M f}) 
-   {r'. \<exists>r. r \<in>rs2 \<and> r'=absTransfRule M r} i s \<longrightarrow> formEval (constrInv f 0 1) s"
-    and a8:"\<forall>s i f. reachableUpTo Is rs2 i s\<longrightarrow> f\<in>F \<longrightarrow>
-    (\<forall>v. v\<in> varOfForm (constrInv f 0 1) \<longrightarrow> s v = (abs1 M s) v) " and
-    a9:"\<forall>r'. r'\<in>rs2 \<longrightarrow> ((\<exists>r f i . f \<in>F  \<and> r \<in>rs \<and>i\<le>N  \<and> 
-  r'=  (strengthenRule2 (constrInvByExcl f i  N) r))| r' \<in>rs)" and
-    a10:"symProtRules' N rs2" and
-    a11:"\<forall>r. r\<in>rs \<longrightarrow> 
-  ((\<exists> f . f \<in>(constrInvByExcls F  N)  \<and>   (strengthenRule2 f r)\<in>rs2)| r \<in>rs2)"
-    and a12:"1 \<le>N "
-    (* ({r'. \<exists>r. r \<in>({r'. (\<exists>r f. f \<in>(F N) \<and> r \<in>rs \<and> r'=  (strengthenRule2 f r))| r'\<in>rs})
-   \<and> r'=absTransfRule M r})*)
-  shows "\<forall>f s  . f\<in>constrInvByExcls F  N \<longrightarrow> reachableUpTo Is rs k s   
-    \<longrightarrow>formEval f s"
-  
-proof((rule allI)+,(rule impI)+)
+  assumes a1: "\<And>r. r \<in> rs \<longrightarrow> wellFormedRule N r"
+    and a2: "\<forall>f. f \<in> F \<longrightarrow> symPair f N"
+    and a3: "symProtRules' N rs" 
+    and a4: "symPredSet' N Is"
+    and a5: "M \<le> N"
+    and a7: "\<forall>i f s. f \<in> F \<longrightarrow> reachableUpTo {f'. \<exists>f. f \<in> Is \<and> f' = absTransfForm M f}
+                {r'. \<exists>r. r \<in> rs2 \<and> r' = absTransfRule M r} i s \<longrightarrow> formEval (constrInv f 0 1) s"
+    and a8: "\<forall>s i f. reachableUpTo Is rs2 i s \<longrightarrow> f \<in> F \<longrightarrow>
+                (\<forall>v. v \<in> varOfForm (constrInv f 0 1) \<longrightarrow> s v = abs1 M s v)"
+    and a9: "\<forall>r'. r' \<in> rs2 \<longrightarrow> ((\<exists>r f i. f \<in> F \<and> r \<in> rs \<and> i \<le> N \<and>
+                r' = (strengthenRule2 (constrInvByExcl f i N) r)) \<or> r' \<in> rs)"
+    and a10: "symProtRules' N rs2"
+    and a11: "\<forall>r. r \<in> rs \<longrightarrow> ((\<exists>f. f \<in> constrInvByExcls F N \<and> strengthenRule2 f r \<in> rs2) \<or> r \<in> rs2)"
+    and a12: "1 \<le> N"
+  shows "\<forall>f s. f \<in> constrInvByExcls F N \<longrightarrow> reachableUpTo Is rs k s \<longrightarrow> formEval f s"
+proof ((rule allI)+,(rule impI)+)
   fix f s  
   assume b0:"f \<in> constrInvByExcls F  N" and b0':" reachableUpTo Is rs k s"  
-  (*let ?rs1=" ({r'. \<exists>r f. f \<in>(F N) \<and> r \<in>rs \<and> r'=  (strengthenRule f r)})"*)
-  let ?rs2=" ({r'. (\<exists>r f i j . f \<in>F \<and>i\<le>N \<and>j\<le>N \<and> r \<in>rs \<and> 
-  r'=  (strengthenRule2 (constrInvByExcl f i  N) r))| r' \<in>rs})"
- 
-  have b1:"\<forall>i f s. f\<in>F \<longrightarrow> reachableUpTo Is rs2 i s \<longrightarrow> formEval (constrInv f 0 1) (abs1 M s)"
-  proof((rule allI)+,(rule impI)+)
+  let ?rs2="({r'. (\<exists>r f i j. f \<in> F \<and> i \<le> N \<and> j \<le> N \<and> r \<in> rs \<and> 
+              r' = (strengthenRule2 (constrInvByExcl f i N) r)) \<or> r' \<in> rs})"
+
+  have b1: "\<forall>i f s. f \<in> F \<longrightarrow> reachableUpTo Is rs2 i s \<longrightarrow> formEval (constrInv f 0 1) (abs1 M s)"
+  proof ((rule allI)+,(rule impI)+)
     fix i f s
-    assume c1:"f \<in>F " and c0:"reachableUpTo Is rs2 i s"
-    have c2:"predSimSet Is ({f'. \<exists>f. f \<in>Is \<and> f'=absTransfForm M f})  M"
+    assume c1: "f \<in> F" and c0: "reachableUpTo Is rs2 i s"
+    have c2: "predSimSet Is ({f'. \<exists>f. f \<in>Is \<and> f'=absTransfForm M f})  M"
       by (smt absTransfFormSim1(2) evalDontCareForm mem_Collect_eq predSimSet_def predSim_def)
 
-    have c3: "transSimRules rs2 
-     ({r'. \<exists>r. r \<in>rs2 \<and> r'=absTransfRule M r}) M"
-    proof(unfold transSimRules_def,rule ballI)
+    have c3: "transSimRules rs2 {r'. \<exists>r. r \<in> rs2 \<and> r' = absTransfRule M r} M"
+    proof (unfold transSimRules_def,rule ballI)
       fix r
-      assume d1:"r \<in> rs2"
-      show "\<exists>r'\<in>{r'. \<exists>r. r \<in> rs2 \<and>
-                       r' = absTransfRule M r}.
-            transSimRule r r' M "
-      proof(rule_tac x=" absTransfRule M r" in bexI)
+      assume d1: "r \<in> rs2"
+      show "\<exists>r' \<in> {r'. \<exists>r. r \<in> rs2 \<and> r' = absTransfRule M r}. transSimRule r r' M "
+      proof (rule_tac x=" absTransfRule M r" in bexI)
         show "transSimRule r (absTransfRule M r) M"
-        proof(rule absRuleSim,cut_tac a5,simp)
+        proof (rule absRuleSim,cut_tac a5,simp)
           show "wellFormedRule N r"
             using a9 d1 local.a1 strengthenRule2Keep by auto
         qed
       next
         show "absTransfRule M r\<in> {r'. \<exists>r. r \<in> rs2 \<and> r' = absTransfRule M r}  "
           using d1 by blast
-        
-        
       qed
     qed
 
-           
-    have c4:" reachableUpTo ({f'. \<exists>f. f \<in>Is \<and> f'=absTransfForm M f}) 
-     ({r'. \<exists>r. r \<in>rs2 \<and> r'=absTransfRule M r}) i (abs1 M s)" thm transSimRulesReachable
-    proof(rule_tac ?fs1.0="Is" and ?rs1.0="rs2"  in  transSimRulesReachable)
-      show " predSimSet Is {f'. \<exists>f. f \<in> Is \<and> f' = absTransfForm M f} M"
+    have c4: "reachableUpTo {f'. \<exists>f. f \<in> Is \<and> f' = absTransfForm M f}
+      {r'. \<exists>r. r \<in> rs2 \<and> r' = absTransfRule M r} i (abs1 M s)"
+    proof (rule_tac ?fs1.0="Is" and ?rs1.0="rs2" in transSimRulesReachable)
+      show "predSimSet Is {f'. \<exists>f. f \<in> Is \<and> f' = absTransfForm M f} M"
         using c2 by blast
     next
-      show " transSimRules rs2 {r'. \<exists>r. r \<in> rs2 \<and> r' = absTransfRule M r} M"
+      show "transSimRules rs2 {r'. \<exists>r. r \<in> rs2 \<and> r' = absTransfRule M r} M"
        using c3 by blast
-     
     next
-      show " reachableUpTo Is  rs2 i s"
+      show "reachableUpTo Is rs2 i s"
         using c0 by blast
     qed
-
     show "formEval (constrInv f 0 1) (abs1 M s)" 
-      using a7 c1 c4  by blast
+      using a7 c1 c4 by blast
   qed
 
-  
-  have b3:"\<forall>s i  f . f\<in>F \<longrightarrow> reachableUpTo Is rs2 i s \<longrightarrow> formEval (constrInv f 0 1) ( s)"
+  have b3: "\<forall>s i f. f \<in> F \<longrightarrow> reachableUpTo Is rs2 i s \<longrightarrow> formEval (constrInv f 0 1) s"
     using a8 absDontAffect b1 by blast
-   
-    
- (* have b4:"\<exists>p f0. f0 \<in> F \<and> p permutes {i. i\<le>N } \<and> equivForm   f   (applySym2Form p f0)"
-    using a2 b0 by blast*)
-
-  (*then obtain p f0 where b5:"f0 \<in> (F M) \<and> p permutes {i. i\<le>N } \<and> f=applySym2Form p f0 "
-    by blast*)
-
-  (*have b5:"symProtRules N rs2" thm symStrengthenRule2
-  proof(rule symStrengthenRule2)
-    show "symProtRules N rs"
-      using a3 by blast
-    show " symPredSet N (F N)"
-      using a6 by blast
-  qed*)
-
       
-      
-  have b6:"\<forall>i s f i' . reachableUpTo Is rs2 i s \<longrightarrow> f\<in>constrInvByExcls F  N \<longrightarrow>
-    i'\<le>N  -->formEval f s"
-  proof((rule allI)+,(rule impI)+)
+  have b6: "\<forall>i s f i'. reachableUpTo Is rs2 i s \<longrightarrow> f \<in> constrInvByExcls F N \<longrightarrow> i' \<le> N \<longrightarrow> formEval f s"
+  proof ((rule allI)+,(rule impI)+)
     fix i s f i'  
-    assume c1:"reachableUpTo Is rs2 i s  " and
-    c2:"f\<in>constrInvByExcls F  N" and c3:"i'\<le>N"  
+    assume c1: "reachableUpTo Is rs2 i s"
+      and c2: "f \<in> constrInvByExcls F N"
+      and c3: "i' \<le> N"
 
-    from c2 have c3:"\<exists>i p. i\<le>N \<and>p \<in> F \<and> f= (constrInvByExcl p i N)"
-      by auto 
+    from c2 have c3: "\<exists>i p. i \<le> N \<and> p \<in> F \<and> f = constrInvByExcl p i N"
+      by (auto simp add: constrInvByExcl_def)
 
-    then obtain i p  where c5:"i\<le>N \<and>p \<in> F \<and> f= (constrInvByExcl p i N)"
-    by blast
+    then obtain i p where c5: "i \<le> N \<and> p \<in> F \<and> f = constrInvByExcl p i N"
+      by blast
 
-    (*have c6:"formEval f0 s"
-      using a8 absDontAffect b1 c1 c5 by blast
-    have c7:"formEval (applySym2Form p f0) s"  
-      apply(rule_tac fs="Is" and rs="rs2" in SymLemma')
-      apply(cut_tac a4,blast)
-      using a10 apply blast
-      using a8 absDontAffect b1 c5 apply blast
-      using c5 apply blast
-      using c1 apply blast
-      done*)
-    show "formEval  f s"
-      apply(cut_tac c5,simp only:c5) thm SymLemmaOnExcl
-      apply(rule_tac Is="Is"  and rs="rs2" in  SymLemmaOnExcl)
+    show "formEval f s"
+      apply (cut_tac c5,simp only:c5)
+      apply (rule_tac Is="Is" and rs="rs2" in SymLemmaOnExcl)
       using a4 apply blast
       using a10 apply blast
-      apply(cut_tac a12) apply force
+      apply (cut_tac a12) apply force
       using a2 c5 apply blast 
       using c1 apply simp
       using a8 absDontAffect b1 c1 c5 apply blast
       using c5 by blast 
-  qed    
-  thm strengthenProt2SimProt
+  qed
   
-  have c7:"\<forall>i s. reachableUpTo Is rs i s \<longrightarrow> 
-  reachableUpTo Is rs2 i s \<and> (\<forall>f. f \<in> constrInvByExcls F  N \<longrightarrow> formEval f s)"
-  proof(rule allI, rule strengthenProt2SimProt,cut_tac a11,blast)
+  have c7: "\<forall>i s. reachableUpTo Is rs i s \<longrightarrow> 
+    reachableUpTo Is rs2 i s \<and> (\<forall>f. f \<in> constrInvByExcls F  N \<longrightarrow> formEval f s)"
+  proof (rule allI, rule strengthenProt2SimProt,cut_tac a11,blast)
     fix i
-    show "\<forall>i s f.
-            reachableUpTo Is rs2 i s \<longrightarrow>
-             f \<in> constrInvByExcls F N \<longrightarrow> formEval f s"
+    show "\<forall>i s f. reachableUpTo Is rs2 i s \<longrightarrow> f \<in> constrInvByExcls F N \<longrightarrow> formEval f s"
       using b6 by blast
   qed
 
   show "formEval f s"
-    using b0 b0' c7 by blast
-    
-qed    
-  
+    using b0 b0' c7 by blast    
+qed
+
+subsection \<open>Auxiliary lemmas\<close>
+
+text \<open>For showing invariants by hand, usually type correctness\<close>
+
+lemma invIntro:
+  assumes "\<And>s0. (\<forall>f\<in>fs. formEval f s0) \<Longrightarrow> Inv s0"
+    and "\<And>r sk. r \<in> rs \<Longrightarrow> formEval (pre r) sk \<Longrightarrow> Inv sk \<Longrightarrow> Inv (trans1 (act r) sk)"
+  shows "reachableUpTo fs rs k s \<Longrightarrow> Inv s"
+proof (induct k arbitrary: s)
+  case 0
+  then show ?case
+    apply (elim reachableUpTo0)
+    using assms(1) by auto
+next
+  case (Suc k)
+  show ?case
+    using Suc(2)
+    apply (elim reachableUpToSuc)
+    subgoal for s' g a
+      using Suc.hyps assms(2) by fastforce
+    done
+qed
+
 end
